src/Example.Check.Simple.fst
@@ -27,58 +27,17 @@ let count_when (p: s bool): s int =
 (* forall e. count_when false <= count_when e <= count_when true *)
 let count_when_prop (e: s bool): s unit =
   let' (count_when ff) (fun count_when_false ->
-  let' (count_when e) (fun count_when_e ->
+  let' (count_when  e) (fun count_when_e ->
   let' (count_when tt) (fun count_when_true ->
-  check' "count_when false <= count_when e" (count_when_false <=^ count_when_e) (
-  check' "cwe<=cwt" (count_when_e <=^ count_when_true) (
-  pure ())))))
-
-let run (e: s 'a) : Exp.exp [] 'a =
-  let (a, _) = e { fresh = 0 } in
-  a
-
-let count (): s int =
-  rec' (fun count -> fby 0 count +^ z1)
-
-let count_when__0_prop (e: s bool): s unit =
-  check' "0 <= count_when e" (z0 <=^ z1) (pure ())
-
+  check' "0                <= count_when false" (z0               <=^ count_when_false) (
+  check' "count_when false <= count_when e"     (count_when_false <=^ count_when_e) (
+  check' "count_when e     <= count_when true"  (count_when_e     <=^ count_when_true) (
+  pure ()))))))
 
 let sys =
-  system_of_exp (run (count_when__0_prop ff))
+  system_of_exp (run1 count_when_prop)
 
-// #push-options "--print_full_names --print_bound_var_types"
-// let prove (fv: sem_freevars): Lemma (ensures base_case (sys fv)) =
-//   assert (base_case (sys fv)) by (T.norm [primops; iota; delta; zeta; nbe]; T.dump "")
-//   // assert (base_case (sys fv)) by (tac_nbe (); T.dump "")
-
-
-
-// let doit (): unit =
-//   let xe = run (count_when_prop (fresh bool)) in
-
-//   assert (xe == Exp.XVal ()) by (T.norm [primops; iota; delta; zeta; nbe]; T.norm [delta_fully ["Pipit.SugarX3.STREAM?.reflect"]]; T.dump "")
-//   // by (tac_nbe (); T.dump "")
-
-
-let sdf (): unit =
-  let xe = run z1 in
-  let xy = run z1 in
-  assert (xe == xy) by (T.norm [primops; iota; delta; nbe]; T.dump "")
-  // by (tac_nbe (); T.dump "")
-
-
-//   let open Sugar in
-//   system_of_exp (
-//     let' (count_when ff) (
-//       let' (count_when x0) (
-//         let' (count_when tt) (
-//           let count_when_false = x2 in
-//           let count_when_e = x1 in
-//           let count_when_true = x0 in
-//           count_when_false <=^ count_when_e /\ count_when_e <=^ count_when_true))))
-//     1
-
-// let count_when_prop_prove (): Lemma (ensures induct1' count_when_prop) =
-//   assert (base_case' count_when_prop) by tac_nbe ();
-//   assert (step_case' count_when_prop) by tac_nbe ()
+#push-options "--print_full_names --print_bound_var_types"
+let prove (fv: sem_freevars): Lemma (ensures induct1 (sys fv)) =
+  assert (base_case (sys fv)) by (tac_nbe (); T.dump "base");
+  assert (step_case (sys fv)) by (tac_nbe (); T.dump "step")
