src/Example.Compile.Pump.fst
@@ -12,11 +12,13 @@ module Tac = FStar.Tactics
 module B   = LowStar.Buffer
 open FStar.HyperStack.ST
 
+module Sugar = Pipit.SugarX4
+
 (* We will translate the controller node with variables as input.
    We do not want the expression's internal representation to show up in the
    C code, so we mark it as noextract. *)
 noextract
-let expr = (Pump.controller (Exp.XVar 0) (Exp.XVar 1) false)
+let expr = Sugar.run2 Pump.controller'
 
 (* Define the state type so it shows up as a type definition in the C code.
    The "postprocess_with" annotation ensures that the state_of_exp is inlined into the type and simplified to a regular type *)
@@ -35,9 +37,10 @@ type output = {
 
 (* Translate the expression to a transition system. *)
 noextract
-let system: Pipit.Exec.Base.exec (int * (int * unit)) state int =
-  assert_norm (Exp.wf expr 2);
-  XX.exec_of_exp expr 2
+let system: Pipit.Exec.Exp.xexec expr =
+  // assert_norm (Exp.wf expr 2);
+  assert_norm (XX.extractable expr);
+  XX.exec_of_exp expr
 
 (* Define the reset function, which takes a pointer to the internal state and
    initialises it. *)
@@ -53,9 +56,21 @@ let has_bit (i: int) (b: nat { b > 0 }) =
    internal state, and returns the result as a bitfield. We parse the bitfield
    before returning the values.
    *)
+
+// [@@(Tac.postprocess_with XL.tac_extract)]
+// let step (inp: input) (stref: B.pointer state): ST output
+//     (requires (fun h -> B.live h stref))
+//     (ensures (fun h _ h' -> B.live h' stref)) =
+//   let res = XL.mk_step system (inp.estop, (inp.level_low, ())) stref in
+//   admit ()
+//   { sol_en = has_bit res Pump.solenoid_flag; nok_stuck = has_bit res Pump.stuck_flag }
+
 [@@(Tac.postprocess_with XL.tac_extract)]
-let step (inp: input) (stref: B.pointer state): ST output
-    (requires (fun h -> B.live h stref))
-    (ensures (fun h _ h' -> B.live h' stref)) =
-  let res = XL.mk_step system (Exp.value_of_bool inp.estop, (Exp.value_of_bool inp.level_low, ())) stref in
-  { sol_en = has_bit res Pump.solenoid_flag; nok_stuck = has_bit res Pump.stuck_flag }
+let step_run (inp: input) = XL.mk_step system (inp.estop, (inp.level_low, ()))
+
+// let step inp s // : ST int
+//     // (requires (fun h -> B.live h stref))
+//     // (ensures (fun h _ h' -> B.live h' stref)) =
+//     =
+//   step_run inp s
+  // admit () // { sol_en = has_bit res Pump.solenoid_flag; nok_stuck = has_bit res Pump.stuck_flag }
