src/Pipit.System.Base.fst
@@ -71,11 +71,11 @@ let prop_holds (p: prop): prop = p
 let system_check (#input #state: Type) (name: string)
   (t1: system input state xprop):
        system input (xprop & state) xprop =
-  { init = (fun (chck, s) -> chck = true /\ t1.init s);
-    step = (fun i (_, s) (chck', s') r ->
-        t1.step i s s' r /\
-        r = chck');
-    chck = (name, (fun (chck, s) -> chck == true)) :: map_checks snd t1.chck;
+  { init = (fun s -> fst s = true /\ t1.init (snd s));
+    step = (fun i s s' r ->
+        t1.step i (snd s) (snd s') r /\
+        r = fst s');
+    chck = (name, (fun s -> fst s == true)) :: map_checks snd t1.chck;
   }
 
 let system_ap2 (#input #state1 #state2 #value1 #value2: Type)
@@ -83,11 +83,11 @@ let system_ap2 (#input #state1 #state2 #value1 #value2: Type)
   (t2: system input state2 value1):
        system input (state1 & state2) value2 =
   {
-    init = (fun (s1, s2) -> t1.init s1 /\ t2.init s2);
-    step = (fun i (s1, s2) (s1', s2') r ->
+    init = (fun s -> t1.init (fst s) /\ t2.init (snd s));
+    step = (fun i s s' r ->
       exists (f: value1 -> value2) (a: value1).
-        t1.step i s1 s1' f /\
-        t2.step i s2 s2' a /\
+        t1.step i (fst s) (fst s') f /\
+        t2.step i (snd s) (snd s') a /\
         r == f a);
     chck =
       app_checks (map_checks fst t1.chck) (map_checks snd t2.chck);
@@ -122,25 +122,40 @@ let rec system_map_sem (#input #state1 #value1 #result: Type) (f: value1 -> resu
 let system_pre (#input #state1 #v: Type) (init: v)
   (t1: system input state1 v):
        system input (state1 & v) v =
-  { init = (fun (s1, v) -> t1.init s1 /\ v == init);
-    step = (fun i (s1, v) (s1', v') r ->
-      t1.step i s1 s1' v' /\ r == v);
+  { init = (fun s -> t1.init (fst s) /\ snd s == init);
+    step = (fun i s s' r ->
+      t1.step i (fst s) (fst s') (snd s') /\ r == snd s);
     chck = map_checks fst t1.chck;
   }
+
+type system_then_state (state1 state2: Type) = {
+  init: bool; s1: state1; s2: state2;
+}
 
 let system_then (#input #state1 #state2 #v: Type)
   (t1: system input state1 v)
   (t2: system input state2 v):
-       system input (bool & state1 & state2) v =
-  { init = (fun (init,s1,s2) -> init = true /\ t1.init s1 /\ t2.init s2);
-    step = (fun i (init,s1,s2) (init',s1',s2') r ->
+       system input (system_then_state state1 state2) v =
+  { init = (fun s ->
+     let init = s.init in
+     let s1 = s.s1 in
+     let s2 = s.s2 in
+     init = true /\ t1.init s1 /\ t2.init s2);
+    step = (fun i s s' r ->
+     let init = s.init in
+     let init' = s'.init in
+     let s1 = s.s1 in
+     let s1' = s'.s1 in
+     let s2 = s.s2 in
+     let s2' = s'.s2 in
+
      if init
      then exists r'. t1.init s1 /\ t1.step i s1 s1' r /\ t2.step i s2 s2' r' /\ init' = false
      else init' = false /\ t2.step i s2 s2' r);
     chck = app_checks
       // Maybe we could relax this to something like "i ==> s1'" as the check for t1 only needs to hold on the first step...
-      (map_checks (fun (i,s1,s2) -> s1) t1.chck)
-      (map_checks (fun (i,s1,s2) -> s2) t2.chck);
+      (map_checks (fun s -> s.s1) t1.chck)
+      (map_checks (fun s -> s.s2) t2.chck);
   }
 
 let system_mu (#input #input' #state1 #v: Type)
@@ -157,8 +172,12 @@ let system_let (#input #input' #state1 #state2 #v1 #v2: Type)
   (t1: system input  state1 v1)
   (t2: system input' state2 v2):
        system input (state1 & state2) v2 =
-  { init = (fun (s1, s2) -> t1.init s1 /\ t2.init s2);
-    step = (fun i (s1, s2) (s1', s2') r ->
+  { init = (fun s -> t1.init (fst s) /\ t2.init (snd s));
+    step = (fun i s s' r ->
+      let s1 = fst s in
+      let s1' = fst s' in
+      let s2 = snd s in
+      let s2' = snd s' in
       exists (r1: v1).
         t1.step i s1 s1' r1 /\
         t2.step (extend i r1) s2 s2' r);
@@ -173,6 +192,7 @@ let system_contract_instance (#input #input_b #input_ab #state1 #state2 #state3 
   (guar: system input_ab state2 prop)
   (arg:  system input    state3 b):
        system input (state1 & state2 & state3) a =
+  // TODO no pattern match
   { init = (fun (s1, s2, s3) -> assm.init s1 /\ guar.init s2 /\ arg.init s3);
     step = (fun i (s1, s2, s3) (s1', s2', s3') r ->
       exists (rb: b). True);
