src/Pipit.System.Det.fst
@@ -4,6 +4,8 @@ module Pipit.System.Det
 open Pipit.System.Base
 module C = Pipit.Context
 
+open Pipit.Inhabited
+
 (* Deterministic systems can't express the whole language, but they can do a subset of it much simpler *)
 noeq
 type dsystem (input: Type) (state: Type) (result: Type) = {
@@ -47,10 +49,10 @@ let dsystem_check (#input #state: Type) (name: string)
   (t1: dsystem input state xprop):
        dsystem input (xprop & state) xprop =
   { init = (true, t1.init);
-    step = (fun i (_, s) ->
-        let (s', r) = t1.step i s in
-        ((r, s'), r));
-    chck = (name, (fun (chck, s) -> chck == true)) :: map_checks snd t1.chck;
+    step = (fun i s ->
+        let (s2', r) = t1.step i (snd s) in
+        ((r, s2'), r));
+    chck = (name, (fun s -> fst s == true)) :: map_checks snd t1.chck;
   }
 
 let dsystem_ap2 (#input #state1 #state2 #value1 #value2: Type)
@@ -59,9 +61,9 @@ let dsystem_ap2 (#input #state1 #state2 #value1 #value2: Type)
        dsystem input (state1 & state2) value2 =
   {
     init = (t1.init, t2.init);
-    step = (fun i (s1, s2) ->
-        let (s1', f) = t1.step i s1 in
-        let (s2', a) = t2.step i s2 in
+    step = (fun i s ->
+        let (s1', f) = t1.step i (fst s) in
+        let (s2', a) = t2.step i (snd s) in
         ((s1', s2'), f a));
     chck =
       app_checks (map_checks fst t1.chck) (map_checks snd t2.chck);
@@ -84,24 +86,40 @@ let dsystem_pre (#input #state1 #v: Type) (init: v)
   (t1: dsystem input state1 v):
        dsystem input (state1 & v) v =
   { init = (t1.init, init);
-    step = (fun i (s1, v) ->
-      let (s1', v') = t1.step i s1 in
-      ((s1', v'), v));
+    step = (fun i s ->
+      let (s1', v') = t1.step i (fst s) in
+      ((s1', v'), snd s));
     chck = map_checks fst t1.chck;
   }
 
 let dsystem_then (#input #state1 #state2 #v: Type)
   (t1: dsystem input state1 v)
   (t2: dsystem input state2 v):
-       dsystem input (bool & state1 & state2) v =
-  { init = (true, t1.init, t2.init);
-    step = (fun i (init,s1,s2) ->
+       dsystem input (system_then_state state1 state2) v =
+  { init = ({ init = true; s1 = t1.init; s2 = t2.init; } <: system_then_state state1 state2);
+    step = (fun i (s: system_then_state state1 state2) ->
+     let init = s.init in
+     let s1 = s.s1 in
+     let s2 = s.s2 in
      let (s1', v1) = t1.step i t1.init in
      let (s2', v2) = t2.step i s2 in
-     ((false, s1', s2'), (if init then v1 else v2)));
+     let s' = { init = false; s1 = s1'; s2 = s2' } <: system_then_state state1 state2 in
+     (s', (if init then v1 else v2)));
     chck = app_checks
-      (map_checks (fun (i,s1,s2) -> s1) t1.chck)
-      (map_checks (fun (i,s1,s2) -> s2) t2.chck);
+      (map_checks (fun s -> s.s1) t1.chck)
+      (map_checks (fun s -> s.s2) t2.chck);
+  }
+
+let dsystem_mu_causal (#input #input' #state1 #v: Type)
+  {| inhabited v |}
+  (extend: input -> v -> input')
+  (t1: dsystem input' state1 v):
+       dsystem input state1 v =
+  { init = t1.init;
+    step = (fun i s ->
+      let (s',r) = t1.step (extend i (get_inhabited <: v)) s in
+      t1.step (extend i r) s);
+    chck = t1.chck;
   }
 
 let dsystem_let (#input #input' #state1 #state2 #v1 #v2: Type)
@@ -110,9 +128,9 @@ let dsystem_let (#input #input' #state1 #state2 #v1 #v2: Type)
   (t2: dsystem input' state2 v2):
        dsystem input (state1 & state2) v2 =
   { init = (t1.init, t2.init);
-    step = (fun i (s1, s2) ->
-      let (s1', r1) = t1.step i s1 in
-      let (s2', r2) = t2.step (extend i r1) s2 in
+    step = (fun i s ->
+      let (s1', r1) = t1.step i (fst s) in
+      let (s2', r2) = t2.step (extend i r1) (snd s) in
       ((s1', s2'), r2));
     chck = app_checks (map_checks fst t1.chck) (map_checks snd t2.chck);
   }
